Proved pure weakening

Gt3/JEq/Basic.lean
@@ -18,7 +18,7 @@ inductive Ctx.JEq : Ctx → Tm 0 → Tm 0 → Tm 0 → Prop
     (hA : JEq Γ (.univ m) A A')
     (hB : ∀ x ∉ L, JEq (Γ.cons x A) (.univ n) (B.open x) (B'.open x))
     (hm : m ≤ ℓ) (hn : n ≤ ℓ) (hℓ : 1 ≤ ℓ)
-  : JEq Γ (.univ (max m n)) (.pi A B) (.pi A' B')
+    : JEq Γ (.univ ℓ) (.pi A B) (.pi A' B')
   | abs {Γ : Ctx} {A A' : Tm 0} {B B' b b' : Tm 1} {t t' : Tm 1} {m n : ℕ} {L : Finset String}
     (hA : JEq Γ (.univ m) A A')
     (hB : ∀ x ∉ L, JEq (Γ.cons x A) (.univ n) (B.open x) (B'.open x))
@@ -63,9 +63,33 @@ inductive Ctx.JEq : Ctx → Tm 0 → Tm 0 → Tm 0 → Prop
 
 def Ctx.WfEq (Γ : Ctx) (a b : Tm 0) : Prop := ∃A, JEq Γ A a b
 
+theorem Ctx.WfEq.symm {Γ a b} (h : WfEq Γ a b) : WfEq Γ b a :=
+  have ⟨A, h⟩ := h; ⟨A, h.symm⟩
+
 def Ctx.IsWf (Γ : Ctx) (a : Tm 0) : Prop := WfEq Γ a a
 
+theorem Ctx.WfEq.lhs {Γ a b} (h : WfEq Γ a b) : IsWf Γ a :=
+  have ⟨A, h⟩ := h; ⟨A, h.trans h.symm⟩
+
+theorem Ctx.WfEq.rhs {Γ a b} (h : WfEq Γ a b) : IsWf Γ b := h.symm.lhs
+
 def Ctx.TyEq (Γ : Ctx) (A B : Tm 0) : Prop := ∃ℓ, JEq Γ (.univ ℓ) A B
+
+theorem Ctx.TyEq.cast {Γ A B} (h : TyEq Γ A B) {a b} (hab : JEq Γ A a b)
+  : JEq Γ B a b := have ⟨_, h⟩ := h; h.cast hab
+
+theorem Ctx.TyEq.symm {Γ A B} (h : TyEq Γ A B) : TyEq Γ B A :=
+  have ⟨ℓ, h⟩ := h; ⟨ℓ, h.symm⟩
+
+theorem Ctx.JEq.cast_level_le {ℓ ℓ' : ℕ} (hℓ : ℓ ≤ ℓ') {Γ A B}
+  (hAB : JEq Γ (.univ ℓ) A B) : JEq Γ (.univ ℓ') A B := by
+  induction hℓ with
+  | refl => assumption
+  | step => apply cast_level; assumption
+
+theorem Ctx.TyEq.trans {Γ A B C} (hAB : TyEq Γ A B) (hBC : TyEq Γ B C) : TyEq Γ A C :=
+  have ⟨n, hAB⟩ := hAB; have ⟨m, hBC⟩ := hBC;
+  ⟨n ⊔ m, (hAB.cast_level_le (by simp)).trans (hBC.cast_level_le (by simp))⟩
 
 def Ctx.IsTy (Γ : Ctx) (A : Tm 0) : Prop := TyEq Γ A A
 
@@ -73,7 +97,11 @@ theorem Ctx.TyEq.wf {Γ A B} (h : TyEq Γ A B) : WfEq Γ A B := have ⟨_, h⟩ 
 
 theorem Ctx.IsTy.wf {Γ A} (h : Ctx.IsTy Γ A) : Ctx.IsWf Γ A := TyEq.wf h
 
-def Ctx.IsSort (Γ : Ctx) (A : Tm 0) : Prop := ∃ℓ, TyEq Γ (.univ ℓ) A
+theorem Ctx.TyEq.lhs {Γ A B} (h : TyEq Γ A B) : IsTy Γ A := h.trans h.symm
+
+theorem Ctx.TyEq.rhs {Γ A B} (h : TyEq Γ A B) : IsTy Γ B := h.symm.lhs
+
+def Ctx.IsUniv (Γ : Ctx) (A : Tm 0) : Prop := ∃ℓ, TyEq Γ (.univ ℓ) A
 
 def Ctx.HasTy' (Γ : Ctx) (A : Tm 0) (a : Tm 0) : Prop := JEq Γ A a a
 
@@ -87,11 +115,21 @@ theorem Ctx.JEq.lhs_is_ty {Γ ℓ A B} (h : JEq Γ (.univ ℓ) A B) : IsTy Γ A 
 
 theorem Ctx.JEq.rhs_is_ty {Γ ℓ A B} (h : JEq Γ (.univ ℓ) A B) : IsTy Γ B := h.rhs_ty'.ty_eq
 
+theorem Ctx.JEq.wf_eq {Γ A a b} (h : JEq Γ A a b) : WfEq Γ a b := ⟨A, h⟩
+
+theorem Ctx.HasTy'.is_wf {Γ A a} (h : HasTy' Γ A a) : IsWf Γ a := ⟨A, h⟩
+
+theorem Ctx.JEq.lhs_is_wf {Γ A a b} (h : JEq Γ A a b) : IsWf Γ a := h.lhs_ty'.is_wf
+
+theorem Ctx.JEq.rhs_is_wf {Γ A a b} (h : JEq Γ A a b) : IsWf Γ b := h.rhs_ty'.is_wf
+
 inductive Ctx.Ok : Ctx → Prop
   | nil : Ok .nil
   | cons {Γ : Ctx} {x : String} {A : Tm 0}
   (hΓ : Ok Γ) (hx : x ∉ Γ.dv) (hA : IsTy Γ A)
   : Ok (Γ.cons x A)
+
+attribute [simp] Ctx.Ok.nil
 
 theorem Ctx.JEq.ok {Γ A a b} (h : JEq Γ A a b) : Ok Γ := by
   induction h <;> repeat first | assumption | constructor
@@ -100,12 +138,41 @@ theorem Ctx.TyEq.ok {Γ A B} (h : TyEq Γ A B) : Ok Γ := have ⟨_, h⟩ := h; 
 
 theorem Ctx.IsTy.ok {Γ A} (h : IsTy Γ A) : Ok Γ := TyEq.ok h
 
+theorem Ctx.Ok.no_dup {Γ} (h : Ok Γ) : NoDup Γ := by induction h <;> constructor <;> assumption
+
+theorem Ctx.Ok.head {Γ x A} (h : Ok (Ctx.cons Γ x A)) : x ∉ Γ.dv ∧ IsTy Γ A
+  := by cases h; simp only [not_false_eq_true, and_self, *]
+
+theorem Ctx.Ok.var {Γ x A} (h : Ok (Ctx.cons Γ x A)) : x ∉ Γ.dv
+  := h.head.left
+
+theorem Ctx.Ok.ty {Γ x A} (h : Ok (Ctx.cons Γ x A)) : IsTy Γ A
+  := h.head.right
+
+theorem Ctx.Ok.tail {Γ x A} (h : Ok (Ctx.cons Γ x A)) : Ok Γ
+  := by cases h; assumption
+
+theorem Ctx.Ok.cons_iff {Γ x A} : Ok (Ctx.cons Γ x A) ↔ Ok Γ ∧ x ∉ Γ.dv ∧ IsTy Γ A
+  := ⟨fun h => ⟨h.tail, h.head⟩, fun ⟨hΓ, hx, hA⟩ => hΓ.cons hx hA⟩
+
 theorem Ctx.JEq.null {Γ} (h : Ok Γ) : JEq Γ .unit .null .null := by
   induction h with
   | nil => exact .nil_ok
   | cons _ _ hA => cases hA; constructor <;> assumption
 
 theorem Ctx.Ok.iff_null {Γ} : JEq Γ .unit .null .null ↔ Ok Γ := ⟨JEq.ok, JEq.null⟩
+
+theorem Ctx.IsTy.univ {Γ ℓ} (h : Ok Γ) : IsTy Γ (.univ ℓ) := ⟨ℓ + 1, .univ (.null h)⟩
+
+theorem Ctx.IsTy.empty {Γ} (h : Ok Γ) : IsTy Γ .empty := ⟨0, .empty (.null h)⟩
+
+theorem Ctx.IsTy.unit {Γ} (h : Ok Γ) : IsTy Γ .unit := ⟨0, .unit (.null h)⟩
+
+@[simp] theorem Ctx.IsTy.univ_iff {Γ ℓ} : IsTy Γ (.univ ℓ) ↔ Ok Γ := ⟨IsTy.ok, IsTy.univ⟩
+
+@[simp] theorem Ctx.IsTy.empty_iff {Γ} : IsTy Γ .empty ↔ Ok Γ := ⟨IsTy.ok, IsTy.empty⟩
+
+@[simp] theorem Ctx.IsTy.unit_iff {Γ} : IsTy Γ .unit ↔ Ok Γ := ⟨IsTy.ok, IsTy.unit⟩
 
 def Ctx.Cmp (Γ : Ctx) (A a b : Tm 0) : Prop := HasTy' Γ A a ∧ HasTy' Γ A b
 
@@ -115,34 +182,4 @@ theorem Ctx.Cmp.symm {Γ A a b} (h : Cmp Γ A a b) : Cmp Γ A b a
 theorem Ctx.Cmp.trans {Γ A a b c} (h : Cmp Γ A a b) (h' : Cmp Γ A b c) : Cmp Γ A a c
   := ⟨h.left, h'.right⟩
 
-theorem Ctx.IsTy.univ {Γ ℓ} (h : Ok Γ) : IsTy Γ (.univ ℓ) := ⟨ℓ + 1, .univ (.null h)⟩
-
-theorem Ctx.IsTy.unit {Γ} (h : Ok Γ) : IsTy Γ .unit := ⟨0, .unit (.null h)⟩
-
-theorem Ctx.IsTy.empty {Γ} (h : Ok Γ) : IsTy Γ .empty := ⟨0, .empty (.null h)⟩
-
 theorem Ctx.JEq.cmp {Γ A a b} (h : JEq Γ A a b) : Cmp Γ A a b := ⟨h.lhs_ty', h.rhs_ty'⟩
-
--- theorem Ctx.Ok.lookup {Γ x A} (h : Ok Γ) (hA : Lookup Γ x A) : IsTy Γ A := by
---   induction hA <;> cases h
-
---TODO: we need weakening!
--- theorem Ctx.JEq.regular {Γ A a b} (h : JEq Γ A a b) : IsTy Γ A := by
---   induction h with
---   | fv => sorry
---   | abs => sorry
---   | app => sorry
---   | nil_ok => sorry
---   | cons_ok => sorry
---   | cast hA => exact hA.rhs_is_ty
---   | _ => first
---     | assumption
---     | constructor; constructor; apply JEq.null; apply IsTy.ok; assumption
-
--- theorem Ctx.JEq.cast_cmp {Γ A B a b} (h : JEq Γ A a b) (h' : Cmp Γ B a b) : JEq Γ B a b := by
---   induction h generalizing B with
---   | fv => exact h'.left
---   | univ => exact h'.left
---   | eqn =>
---     sorry
---   | _ => sorry
