Gt3/JEq/Wk.lean
@@ -1,0 +1,102 @@
+import Gt3.JEq.Basic
+
+structure Ctx.PSub (Γ Δ : Ctx) : Prop where
+  left_ok : Ok Γ
+  right_ok : Ok Δ
+  is_perm : LSub Γ Δ
+
+theorem Ctx.Ok.psub {Γ} (h : Ok Γ) : PSub Γ Γ := ⟨h, h, .refl Γ⟩
+
+theorem Ctx.PSub.trans {Γ Δ Θ} (hΓΔ : PSub Γ Δ) (hΔΘ : PSub Δ Θ) : PSub Γ Θ where
+  left_ok := hΓΔ.left_ok
+  right_ok := hΔΘ.right_ok
+  is_perm := hΓΔ.is_perm.trans hΔΘ.is_perm
+
+theorem Ctx.PSub.dv {Γ Δ} (hΓΔ : PSub Γ Δ) : Δ.dv ⊆ Γ.dv := hΓΔ.is_perm.dv
+
+theorem Ctx.PSub.cons' {Γ Δ} (h : PSub Γ Δ)
+  {x A} (hx : x ∉ Γ.dv) (hΓA : IsTy Γ A) (hΔA : IsTy Δ A)
+  : PSub (Γ.cons x A) (Δ.cons x A) where
+  left_ok := h.left_ok.cons hx hΓA
+  right_ok := h.right_ok.cons (Finset.not_mem_subset h.dv hx) hΔA
+  is_perm := h.is_perm.cons x A
+
+theorem Ctx.JEq.psub {Γ Δ} (h : PSub Γ Δ) {A a b : Tm 0} (hab : JEq Δ A a b)
+  : JEq Γ A a b := by
+  induction hab generalizing Γ with
+  | nil_ok | cons_ok => exact .null h.left_ok
+  | cast_level => apply cast_level; apply_assumption; assumption
+  | cast => apply cast <;> apply_assumption <;> assumption
+  | symm => apply symm; apply_assumption; assumption
+  | trans => apply trans <;> apply_assumption <;> assumption
+  | _ =>
+    constructor <;> first
+    | apply_assumption <;> assumption
+    | {
+      rename Finset String => L
+      intro x hx
+      have ⟨hL, hΓ⟩ : x ∉ L ∧ x ∉ Γ.dv := by rw [<-Finset.notMem_union]; exact hx
+      apply_assumption
+      · exact hL
+      · apply PSub.cons'
+        <;> first | assumption | apply JEq.lhs_is_ty <;> apply_assumption <;> assumption
+    }
+    | apply h.is_perm; assumption
+
+theorem Ctx.TyEq.psub {Γ Δ} (h : PSub Γ Δ) {A B : Tm 0} (hAB : TyEq Δ A B)
+  : TyEq Γ A B := have ⟨ℓ, hAB⟩ := hAB; ⟨ℓ, hAB.psub h⟩
+
+theorem Ctx.IsTy.psub {Γ Δ} (h : PSub Γ Δ) {A : Tm 0} (hA : IsTy Δ A)
+  : IsTy Γ A := TyEq.psub h hA
+
+theorem Ctx.PSub.cons {Γ Δ} (h : PSub Γ Δ)
+  {x A} (hx : x ∉ Γ.dv) (hΔA : IsTy Δ A)
+  : PSub (Γ.cons x A) (Δ.cons x A) where
+  left_ok := h.left_ok.cons hx (hΔA.psub h)
+  right_ok := h.right_ok.cons (Finset.not_mem_subset h.dv hx) hΔA
+  is_perm := h.is_perm.cons x A
+
+theorem Ctx.PSub.skip {Γ Δ} (h : PSub Γ Δ)
+  {x A} (hx : x ∉ Γ.dv) (hΓA : IsTy Γ A)
+  : PSub (Γ.cons x A) Δ where
+  left_ok := h.left_ok.cons hx (hΓA)
+  right_ok := h.right_ok
+  is_perm := h.is_perm.skip (Finset.not_mem_subset h.dv hx) A
+
+theorem Ctx.JEq.wk0 {Γ A a b} (hab : JEq Γ A a b) {x B} (hx : x ∉ Γ.dv) (hB : Γ.IsTy B)
+  : JEq (Γ.cons x B) A a b
+  := hab.psub (hab.ok.psub.skip hx hB)
+
+theorem Ctx.TyEq.wk0 {Γ A B} (hAB : TyEq Γ A B) {x C} (hx : x ∉ Γ.dv) (hC : Γ.IsTy C)
+  : TyEq (Γ.cons x C) A B
+  := hAB.psub (hAB.ok.psub.skip hx hC)
+
+theorem Ctx.IsTy.wk0 {Γ A} (hA : IsTy Γ A) {x B} (hx : x ∉ Γ.dv) (hB : Γ.IsTy B)
+  : IsTy (Γ.cons x B) A
+  := hA.psub (hA.ok.psub.skip hx hB)
+
+theorem Ctx.Ok.lookup {Γ x A} (h : Ok Γ) (hA : Lookup Γ x A) : IsTy Γ A
+  := by induction hA <;> cases h <;> apply IsTy.wk0 <;> apply_assumption; assumption
+
+-- theorem Ctx.JEq.regular {Γ A a b} (h : JEq Γ A a b) : IsTy Γ A := by induction h with
+--   | fv hΓ hA => exact hΓ.ok.lookup hA
+--   | abs =>
+--     --TODO: we need _substitution_ here
+--     sorry
+--   | cons_ok =>
+--     simp only [IsTy.unit_iff, Ok.cons_iff, not_false_eq_true, true_and, *]
+--     constructor
+--     · apply JEq.ok; assumption
+--     · apply JEq.rhs_is_ty; assumption
+--   | _ =>
+--     first | assumption
+--           | (simp [*] <;> apply Ctx.IsTy.ok <;> assumption)
+--           | apply JEq.rhs_is_ty; assumption
+
+-- theorem Ctx.JEq.cast_cmp {Γ A B a b} (h : JEq Γ A a b) (h' : Cmp Γ B a b) : JEq Γ B a b := by
+--   induction h generalizing B with
+--   | fv => exact h'.left
+--   | univ => exact h'.left
+--   | eqn =>
+--     sorry
+--   | _ => sorry
